theories/logrel_heaplang_sessions/rules/arr.v
@@ -5,14 +5,21 @@ From iris.heap_lang Require Import notation proofmode.
 
 Section types.
   Context `{heapG Σ}.
+
+  (* I'm guessing the postcondition doesn't need an additional later
+  for contractiveness since the WP already has one? *)
   Definition lty_arr (A1 A2 : lty Σ) : lty Σ := Lty (λ w,
-    ∀ v, A1 v -∗ WP App w v {{ A2 }})%I.
+    ∀ v, ▷ A1 v -∗ WP App w v {{ A2 }})%I.
 End types.
 
 Infix "→" := lty_arr : lty_scope.
 
 Section properties.
   Context `{heapG Σ}.
+
+  (* Cannot get this instance to work for some reason *)
+  (* Global Instance lty_prod_contractive n : *)
+  (*   Proper (dist_later n ==> dist_later n ==> dist n) (@lty_arr Σ). *)
 
   Global Instance lty_arr_ne : NonExpansive2 (@lty_arr Σ _).
   Proof. solve_proper. Qed.
